CSharpRewrite/CSharpRewrite/Program.cs
@@ -1,0 +1,62 @@
+﻿using System;
+using System.Collections.Generic;
+using System.Diagnostics;
+using System.Linq;
+using System.Text;
+using System.Threading.Tasks;
+
+namespace CSharpRewrite
+{
+    internal class Program
+    {
+        static void Main(string[] args)
+        {
+            var turnstile = new Turnstile(State.Boot, 20.0);
+            var pass = new RiderPass(88884444, 2);
+            var card = new PaymentCard(4444333322221111, 50.0);
+            var falseCard = new PaymentCard(5089689782389771, 50.0);
+
+            turnstile.Initialize();
+
+            Console.WriteLine($"# False Card Test#");
+            bool test = turnstile.ProcessNFCSource(falseCard);
+
+            Console.WriteLine($"Operation completed?: {test}");
+            Debug.Assert(test == false);
+
+            Console.WriteLine($"# Working Pass Test#");
+            Console.WriteLine($"# Rides : {pass.rides} #");
+            bool res1 = turnstile.ProcessNFCSource(pass);
+            Console.WriteLine($"Operation completed?: {res1}");
+            Console.WriteLine($"# Rides : {pass.rides} #");
+            Debug.Assert(pass.rides == 1);
+            
+            bool res2 = turnstile.ProcessNFCSource(pass);
+            Console.WriteLine($"Operation completed?: {res2}");
+            Console.WriteLine($"# Rides : {pass.rides} #");
+            Debug.Assert(pass.rides == 0);
+
+            bool res3 = turnstile.ProcessNFCSource(pass);
+            Console.WriteLine($"Operation completed?: {res3}");
+            Console.WriteLine($"# Rides : {pass.rides} #");
+            Debug.Assert(!res3);
+
+            Console.WriteLine($"# Working Card Test#");
+            Console.WriteLine($"# Balance : {card.balance} #");
+            bool res4 = turnstile.ProcessNFCSource(card);
+            Console.WriteLine($"Operation completed?: {res4}");
+            Console.WriteLine($"# Balance  : {card.balance} #");
+            Debug.Assert(card.balance == 30.0);
+
+            bool res5 = turnstile.ProcessNFCSource(card);
+            Console.WriteLine($"Operation completed?: {res5}");
+            Console.WriteLine($"# Balance  : {card.balance} #");
+            Debug.Assert(card.balance == 10.0);
+
+            bool res6 = turnstile.ProcessNFCSource(card);
+            Console.WriteLine($"Operation completed?: {res6}");
+            Console.WriteLine($"# Balance  : {card.balance} #");
+            Debug.Assert(card.balance == 10.0);
+        }
+    }
+}
