Program.dfy
@@ -5,36 +5,42 @@ method Main()
 {
     var turnstile := new Turnstile(Boot, 20.0); 
     var pass := new RiderPass(88884444, 2);
-    var card := new PaymentCard(5089_6897_8238_9772, 50.0);
+    var card := new PaymentCard(4444_3333_2222_1111, 50.0);
+
+    var falseCard := new PaymentCard(5089_6897_8238_9771, 50.0); 
 
     turnstile.Initialize();
+
+    var test := turnstile.ProcessNFCSource(falseCard);
+
+    expect test == false;
 
     assert pass.rides == 2;
     assert card.balance == 50.0;
 
     var res1 := turnstile.ProcessNFCSource(pass);
-    print res1, "\n";
+    print "Operation completed?: ", res1, "\n";
     assert res1 ==> pass.rides == 1;
     
 
     var res2 := turnstile.ProcessNFCSource(pass);
-    print res2, "\n";
+    print "Operation completed?: ", res2, "\n";
     assert res1 && res2 ==> pass.rides == 0; 
     
 
     var res3 := turnstile.ProcessNFCSource(pass);
-    print res3, "\n";
+    print "Operation completed?: ", res3, "\n";
     assert res1 && res2 ==> !res3;
 
     var res4 := turnstile.ProcessNFCSource(card);
-    print res4, "\n";
+    print "Operation completed?: ", res4, "\n";
     assert res4 ==> card.balance == 30.0;
 
     var res5 := turnstile.ProcessNFCSource(card);
-    print res5, "\n";
+    print "Operation completed?: ", res5, "\n";
     assert res4 && res5 ==> card.balance == 10.0;
 
     var res6 := turnstile.ProcessNFCSource(card);
-    print res6, "\n";
+    print "Operation completed?: ", res6, "\n";
     assert res4 && res5 && !res6 ==> card.balance == 10.0;
 }
